wip on compile_stmt_correct_aux. existentials in conclusion are annoying, and eexists does not help because each case needs a different instantiation

src/FlatToRiscv.v
@@ -1,4 +1,5 @@
 Require Import lib.LibTactics.
+Require Import compiler.StateMonad.
 Require Import compiler.Common.
 Require Import compiler.FlatImp.
 Require Import compiler.StateCalculus.
@@ -53,19 +54,151 @@ Section FlatToRiscv.
     end.
 
   Definition containsProgram(m: RiscvMachine)(program: list (@Instruction var))(offset: word w)
-    := forall i inst, nth_error program i = Some inst -> m.(instructionMem) (offset ^+ $i) = inst.
+    := forall i inst, nth_error program i = Some inst ->
+                      m.(instructionMem) (offset ^+ $4 ^* $i) = inst.
 
   Definition containsState(m: RiscvMachine)(s: state)
     := forall x v, get s x = Some v -> m.(registers) x = v.
 
+  (*
   Definition containsProgramAndState(m: RiscvMachine)(program: list (@Instruction var))(s: state)
     := containsProgram m program m.(pc) /\ containsState m s.
+  *)
 
-  Lemma compile_stmt_correct_aux: forall s insts fuelH initialH finalH initialL,
+  (* TODO define type classes in such a way that this is not needed *)
+  Definition myRiscvMachine := @IsRiscvMachine w var R0 _.
+  Existing Instance myRiscvMachine.
+
+(* inline because the inverison is already done
+  Lemma compile_op_correct: forall x y z fuelH op insts initialH finalH initialL,
+    compile_op x op y z = insts ->
+    eval_stmt fuelH initialH (SOp x op y z) = Success finalH ->
+    containsProgram initialL insts initialL.(pc) ->
+    containsState initialL initialH ->
+    exists (fuelL: nat) (finalL: RiscvMachine),
+      execState (run fuelL) initialL = finalL /\
+      containsState finalL finalH.
+  Proof.
+    introv C EvH Cp Cs.
+    destruct fuelH as [|fuelH]; [discriminate|].
+    simpl in EvH.
+  Abort.
+  *)
+  
+  Axiom wmult_neut_r: forall (sz : nat) (x : word sz), x ^* $0 = $0.
+
+  Lemma containsProgram_cons_inv: forall s inst insts offset,
+    containsProgram s (inst :: insts) offset ->
+    s.(instructionMem) offset = inst /\
+    containsProgram s insts (offset ^+ $4).
+  Proof.
+    introv Cp. unfold containsProgram in Cp. split.
+    + specialize (Cp 0). specializes Cp; [reflexivity|].
+      rewrite wmult_neut_r in Cp.
+      rewrite wplus_comm in Cp. rewrite wplus_unit in Cp.
+      assumption.
+    + unfold containsProgram.
+      intros i inst0 E. specialize (Cp (S i)). simpl in Cp.
+      specialize (Cp _ E).
+      rewrite <- Cp. f_equal.
+      rewrite <- wplus_assoc. f_equal. rewrite (natToWord_S w i).
+      replace ($4 ^* ($1 ^+ $i)) with ((($1 ^+ $i) ^* $4): word w) by apply wmult_comm.
+      rewrite wmult_plus_distr.
+      rewrite wmult_unit.
+      f_equal.
+      apply wmult_comm.
+  Qed.
+
+  Lemma containsState_put: forall prog1 prog2 pc1 pc2 initialH initialRegs x v1 v2,
+    containsState (mkRiscvMachine prog1 initialRegs pc1) initialH ->
+    v1 = v2 ->
+    containsState (mkRiscvMachine prog2 
+      (fun reg2 : var =>
+               if dec (x = reg2)
+               then v1
+               else initialRegs reg2)
+       pc2)
+     (put initialH x v2).
+  Proof.
+    unfold containsState. intros. simpl.
+    rewrite get_put in H1. destruct_one_match.
+    - inversions H1. reflexivity.
+    - simpl in H. apply H. assumption.
+  Qed.
+
+
+  Lemma distr_if_over_app: forall T U P1 P2 (c: sumbool P1 P2) (f1 f2: T -> U) (x: T),
+    (if c then f1 else f2) x = if c then f1 x else f2 x.
+  Proof. intros. destruct c; reflexivity. Qed.
+
+  Lemma pair_eq_acc: forall T1 T2 (a: T1) (b: T2) t,
+    t = (a, b) -> a = fst t /\ b = snd t.
+  Proof. intros. destruct t. inversionss. auto. Qed.
+
+  Lemma compile_stmt_correct_aux: forall fuelH s insts initialH finalH initialL,
     compile_stmt s = insts ->
     eval_stmt fuelH initialH s = Success finalH ->
-    containsProgramAndState initialL insts initialH ->
-    exists fuelL, fuelL = 0 /\ False.
+    containsProgram initialL insts initialL.(pc) ->
+    containsState initialL initialH ->
+    exists (fuelL: nat) (finalL: RiscvMachine),
+      execState (run fuelL) initialL = finalL /\
+      containsState finalL finalH.
+  Proof.
+    induction fuelH; [intros; discriminate |].
+    introv C EvH Cp Cs.
+    invert_eval_stmt.
+    - subst.
+      apply containsProgram_cons_inv in Cp. apply proj1 in Cp.
+      destruct initialL as [initialProg initialRegs initialPc].
+      exists 1. eexists. simpl.
+      split.
+      + cbv [execState StateMonad.put execute instructionMem registers pc].
+        simpl in Cp.
+        rewrite Cp. simpl. reflexivity.
+      + eapply containsState_put; [eassumption|].
+        (* TODO holds if we add the right assumptions *) admit.
+    - simpl in C. subst.
+      destruct initialL as [initialProg initialRegs initialPc].
+      simpl in Cp.
+      unfold containsState in Cs. simpl in Cs.
+      rename H into Gy, H0 into Gz. apply Cs in Gy. apply Cs in Gz.
+      subst x0 x1.
+      destruct op;
+      lazymatch goal with
+      | Cp: containsProgram ?s ?p ?PC |- _ =>
+        let p' := eval simpl in p in
+        change (containsProgram s p' PC) in Cp;
+        let l := eval cbv in (length p') in exists l;
+        eexists; (split;
+        [ cbv [run execState StateMonad.put execute instructionMem registers 
+               pc getPC loadInst setPC getRegister setRegister myRiscvMachine IsRiscvMachine gets
+               StateMonad.get Return Bind State_Monad ];
+          repeat (
+            apply containsProgram_cons_inv in Cp;
+            let Cp' := fresh Cp in 
+            destruct Cp as [Cp' Cp];
+            simpl in Cp'
+          );
+          repeat match goal with
+          | E: ?t = ?rhs |- context [?t] => rewrite E
+          end;
+          simpl;
+          lazymatch goal with
+          | |- mkRiscvMachine _ _ _ = _ => reflexivity
+          | |- _ => idtac
+          end
+        | try (unify l 1; eapply containsState_put; [eassumption|reflexivity]) ])
+      end.
+      { assert (initialRegs R0 ^+ initialRegs R0 = $0) as ER0 by admit. (* TODO *)
+        rewrite ER0.
+        match goal with
+        | |- context [weq ?a ?b] => destruct (weq a b) eqn: E
+        end.
+        - rewrite Cp2. simpl. reflexivity.
+        - (* problem: here we should only have made 2 steps instead of 3 *)
+
+
   Abort.
+
 
 End FlatToRiscv.
